added full parameter to is_allocator

misc-verification/slab_allocator.v
@@ -75,23 +75,27 @@ Section Hoare.
           is_valid_loc l al ∗ is_freelist_rec l1 al s
     end.
     
-  Definition is_freelist fl al : iProp Σ := 
-    fl ↦ NONEV 
-      ∨
-    ∃ l1 size, fl ↦ SOMEV #l1 ∗ is_freelist_rec l1 al size.
+  Definition is_freelist fl al (empty : bool) : iProp Σ := 
+    match empty with 
+    | true => fl ↦ NONEV  
+    | false => ∃ l1 size, fl ↦ SOMEV #l1 ∗ is_freelist_rec l1 al size
+    end. 
 
-  (*might not want bs to be persistant as mimalloc can repurpose a  
-     page to new page queue so new size *)
-  Definition is_allocator (al : loc) bs : iProp Σ := 
-    ∃ (res cap : nat), ⌜res > 0⌝ ∗ ⌜cap ≤ res⌝ ∗ ⌜bs > 0⌝ ∗ (al +ₗ 2) ↦□  #res ∗ 
-      (al +ₗ 3) ↦ #cap ∗ (al +ₗ 4) ↦□  #bs ∗ is_freelist al al ∗ 
-      is_freelist (al +ₗ 1) al ∗
+  Definition is_allocator al bs full: iProp Σ := 
+    ∃ res cap bfl1 bfl2, 
+      ⌜res > 0⌝ ∗ ⌜cap ≤ res⌝ ∗ ⌜bs > 0⌝ ∗ 
+      ⌜full = true <-> res = cap ∧ (bfl1 = true) ∧ (bfl2 = true)⌝ ∗ 
+      (al +ₗ 2) ↦□  #res ∗ 
+      (al +ₗ 3) ↦ #cap ∗ 
+      (al +ₗ 4) ↦□  #bs ∗ 
+      is_freelist al al bfl1 ∗ 
+      is_freelist (al +ₗ 1) al bfl2 ∗
       (al +ₗ (5 + cap * bs)) ↦∗ replicate ((res - cap) * bs) NONEV. 
 
   Lemma new_alloc_hoare res bs : 
     {{{ ⌜res > 0⌝ ∗ ⌜bs > 0⌝ }}} 
       new_alloc #res #bs 
-    {{{ al, RET #al; is_allocator al bs }}}.
+    {{{ al, RET #al; is_allocator al bs false }}}.
   Proof. 
     iIntros (φ) "(%Hn & %Hbs) Hphi". iUnfold new_alloc. wp_pures.
     wp_apply wp_allocN; [lia|done|]. iIntros "%al (HalN & _)". 
@@ -101,65 +105,70 @@ Section Hoare.
     wp_store. rewrite !Loc.add_assoc. wp_store. wp_store. wp_store. iApply "Hphi". 
     iExists res, 0. 
     iMod (pointsto_persist with "Hal2") as "#Hal2". 
-    iMod (pointsto_persist with "Hal4") as "#Hal4". iFrame "Hal Hal1 Hal2 Hal3 Hal4".
-    iSplitR; [by iPureIntro|]. iSplitR; [iPureIntro; lia|]. iSplitR; [by iPureIntro|]. 
+    iMod (pointsto_persist with "Hal4") as "#Hal4". iExists true, true. 
+    iFrame "Hal Hal1 Hal2 Hal3 Hal4". iSplitR; [by iPureIntro|]. iSplitR; 
+    [iPureIntro; lia|]. iSplitR; [by iPureIntro|]. iSplitR; [by iPureIntro; lia|]. 
     by rewrite Z.mul_0_l Nat.sub_0_r.
   Qed.
 
-  Lemma freelist_pop_hoare al fl bs : 
-    {{{ (al +ₗ 4) ↦□ #bs ∗ is_freelist fl al }}} 
+  Lemma freelist_pop_hoare al fl bs b : 
+    {{{ (al +ₗ 4) ↦□ #bs ∗ is_freelist fl al b }}} 
       freelist_pop #fl
     {{{ vret, RET vret; 
-      (⌜vret = NONEV⌝ ∗ fl ↦ NONEV 
+      (⌜vret = NONEV⌝ ∗ is_freelist fl al true
         ∨ 
-      ∃ l, ⌜vret = SOMEV #l⌝ ∗ 
+      ∃ l b', ⌜vret = SOMEV #l⌝ ∗ 
         ([∗ list] i ∈ seq 0 bs, ∃ v, (l +ₗ i) ↦ v) ∗ 
-        is_valid_loc l al ∗ is_freelist fl al)
+        is_valid_loc l al ∗ is_freelist fl al b')
     }}}. 
   Proof.
-    iIntros (φ) "(#Hal4 & [H | (%l1 & %s & Hfl & Hflr)]) Hphi"; 
+    iIntros (φ) "(#Hal4 & Hfl) Hphi". 
+    destruct b; [|iDestruct "Hfl" as "(%l1 & %s & Hfl & Hflr)"]; 
     iUnfold freelist_pop; wp_load; wp_pures.
     { iApply "Hphi". iFrame. by iLeft. }
     destruct s; simpl.
     { iDestruct "Hflr" as "(%bs1 & #Hal4' & Hl1 & Hl1r & #Hl1v)". 
-      wp_load. wp_store. wp_pures. iApply "Hphi". iFrame. iRight. 
-      iExists l1. iFrame. iSplitR; [by iPureIntro|].
-      iCombine "Hal4 Hal4'" gives %[_ Heq]. simplify_eq. simpl. iFrame "Hl1v Hl1r". 
-      iExists NONEV. by rewrite Loc.add_0. }
+      iCombine "Hal4 Hal4'" gives %[_ Heq]. simplify_eq.
+      wp_load. wp_store. wp_pures. iApply "Hphi". iRight. iExists l1, true. iFrame. 
+      iSplitR; [by iPureIntro|]. iFrame "Hl1v". iExists NONEV. by rewrite Loc.add_0. }
     iDestruct "Hflr" as "(%bs1 & #Hal4' & %l & Hl1 & Hl1r & #Hl1v & Hflr)". 
     wp_load. wp_store. wp_pures. iApply "Hphi". 
     iRight. iCombine "Hal4 Hal4'" gives %[_ Heq]. simplify_eq. simpl. 
-    iFrame "Hl1v Hl1r". iSplitR; [by iPureIntro|]. rewrite Loc.add_0. 
-    iSplitL "Hl1"; [auto|]. iRight. by iFrame. 
+    iFrame "Hl1v Hl1r". iExists false. iSplitR; [by iPureIntro|]. rewrite Loc.add_0. 
+    iSplitL "Hl1"; [auto|]. by iFrame. 
   Qed.
 
-  Lemma freelist_push_hoare l fl al : 
+  Lemma freelist_push_hoare l fl al b : 
     {{{ 
       ∃ bs, (al +ₗ 4) ↦□ #(S bs) ∗
-      is_freelist fl al ∗ (([∗ list] i ∈ seq 0 (S bs), ∃ v, (l +ₗ i) ↦ v)) ∗ 
+      is_freelist fl al b ∗ (([∗ list] i ∈ seq 0 (S bs), ∃ v, (l +ₗ i) ↦ v)) ∗ 
       is_valid_loc l al 
     }}}
       freelist_push #fl #l
-    {{{ RET #(); is_freelist fl al }}}.
+    {{{ RET #(); is_freelist fl al false }}}.
   Proof. 
-    simpl. rewrite Loc.add_0. iIntros (φ) "(%bs&#Hal4&[H | (%l1 & %s & Hfl & Hflr)] & 
-    ((%v & Hl) & Hl1bs) & Hlv) Hphi"; iUnfold freelist_push; wp_load; wp_store; 
-    wp_store. { iApply "Hphi". iRight. iFrame. iExists 0. iFrame. by iFrame "Hal4". }
-    iApply "Hphi". iRight. iExists l, (S s). by iFrame. 
+    simpl. rewrite Loc.add_0. iIntros (φ) "(%bs&#Hal4&Hfl&((%v & Hl)&Hl1bs)&#Hlv)Hphi".
+    destruct b; [|iDestruct "Hfl" as "(%l1 & %s & Hfl & Hflr)"]; iUnfold freelist_push; 
+    wp_load; wp_store; wp_store. 
+    { iApply "Hphi". iFrame. iExists 0. iFrame. by iFrame "Hlv Hal4". }
+    iApply "Hphi". iExists l, (S s). iFrame. by iFrame "Hlv Hal4".
   Qed.
 
-  Lemma free_hoare l al bs : 
+  Lemma free_hoare l al bs b : 
     {{{ 
-      is_allocator al (S bs) ∗ (([∗ list] i ∈ seq 0 (S bs), ∃ v, (l +ₗ i) ↦ v)) ∗ 
+      is_allocator al (S bs) b ∗ (([∗ list] i ∈ seq 0 (S bs), ∃ v, (l +ₗ i) ↦ v)) ∗ 
       is_valid_loc l al 
     }}}
       free #al #l
-    {{{ RET #(); is_allocator al (S bs) }}}.
+    {{{ RET #(); is_allocator al (S bs) false }}}.
   Proof.
-    iIntros (φ) "((%res&%cap&%Hr&%Hcr&%Hbs&#Hal2&Hal3&#Hal4&Hfl&Hfl2&Hun)&Hlbs&#Hlv)Hphi".
-    iUnfold free. wp_pures. iApply (freelist_push_hoare with "[Hfl2 Hlbs]").
+    iIntros (φ) "((%res&%cap&%b1&%b2&%Hr&%Hcr&%Hbs&%Hf&#Hal2&Hal3&#Hal4&Hfl&Hfl2&Hun)
+    &Hlbs&#Hlv)Hphi". iUnfold free. wp_pures. 
+    iApply (freelist_push_hoare with "[Hfl2 Hlbs]").
     - iFrame. auto. 
-    - iNext. iIntros "Hfl2". iApply "Hphi". iFrame. auto.
+    - iNext. iIntros "Hfl2". iApply "Hphi". iFrame. iFrame "Hal2 Hal4". 
+      iSplitR; [done|]. iSplitR; [done|]. iSplitR; [done|]. iPureIntro.  
+      intuition; inversion H0.
   Qed.
 
   Lemma seq_array_pointsto_eq l dq v n :
@@ -173,7 +182,7 @@ Section Hoare.
     setoid_rewrite <-Loc.add_assoc; iApply "IH"; done.
   Qed.
 
-  Lemma freelist_extend_hoare fl al res bs lb cap n c d : 
+  Lemma freelist_extend_hoare fl al res bs b lb cap n c d : 
     d = n - c -> 
     lb = (al +ₗ (5 + cap * bs)) ->
     cap ≤ res ->
@@ -181,15 +190,15 @@ Section Hoare.
     bs > 0 ->
     {{{ 
       (al +ₗ 2) ↦□ #res ∗ (al +ₗ 4) ↦□ #bs ∗
-      is_freelist fl al ∗ (lb +ₗ (c * bs)) ↦∗ replicate (d * bs) NONEV 
+      is_freelist fl al b ∗ (lb +ₗ (c * bs)) ↦∗ replicate (d * bs) NONEV 
     }}} 
       freelist_extend #fl #lb #bs #n #c
-    {{{ RET #(); is_freelist fl al }}}. 
+    {{{ RET #(); is_freelist fl al (b && (d =? 0)) }}}. 
   Proof. 
-    iInduction d as [|d IH] forall (c); simpl; 
+    iInduction d as [|d IH] forall (b c); simpl; 
     iIntros (Hd -> Hcr Hd2 Hbs φ) "(#Hal2 & #Hal4 & Hfl & Hun) Hphi"; 
     iUnfold freelist_extend; wp_pures. 
-    { case_bool_decide; [lia|]. wp_pures. by iApply "Hphi". }
+    { case_bool_decide; [lia|]. wp_pures. iApply "Hphi". by rewrite andb_true_r. }
     case_bool_decide; [|lia]. wp_pures. 
     rewrite replicate_add array_app length_replicate. 
     iDestruct "Hun" as "(Hun1 & Hun2)". 
@@ -206,36 +215,49 @@ Section Hoare.
     [lia|done|lia|lia|done| |]. 
     { iFrame "Hal2 Hal4 Hfl". rewrite Loc.add_assoc. 
       by rewrite Nat2Z.inj_add Z.mul_add_distr_r Z.mul_1_l. }
-    iNext. iIntros. by iApply "Hphi".
+    iNext. iIntros. iApply "Hphi". by rewrite andb_false_l andb_false_r.
   Qed. 
 
-  Lemma extend_hoare al bs : 
-    {{{ is_allocator al bs }}} 
+  (*instead of is_allocator al bs as precondition 
+     we have empty freelists, so that we can prove that 
+     something stronger then ∃ b, is_allocator al bs b in post conditoin
+     we need this to prove alloc *)
+  Lemma extend_hoare al res cap bs : 
+    res > 0 -> 
+    cap ≤ res -> 
+    bs > 0 -> 
+    {{{ 
+      (al +ₗ 2) ↦□  #res ∗ (al +ₗ 3) ↦ #cap ∗ (al +ₗ 4) ↦□  #bs ∗ 
+      is_freelist al al true ∗ is_freelist (al +ₗ 1) al true ∗
+      (al +ₗ (5 + cap * bs)) ↦∗ replicate ((res - cap) * bs) NONEV 
+    }}} 
       extend #al 
-      {{{ vret, RET vret; 
-        is_allocator al bs ∗ 
-        ((∃ l, ⌜vret = SOMEV #l⌝ ∗ (([∗ list] i ∈ seq 0 bs, ∃ v, (l +ₗ i) ↦ v)) ∗ 
-          is_valid_loc l al) 
-          ∨  
-        ⌜vret = NONEV⌝)
-      }}}.
+    {{{ vret, RET vret; 
+      ((∃ l, ⌜vret = SOMEV #l⌝ ∗ (([∗ list] i ∈ seq 0 bs, ∃ v, (l +ₗ i) ↦ v)) ∗ 
+        is_valid_loc l al ∗ is_allocator al bs (res - cap =? 1))  
+        ∨  
+      ⌜vret = NONEV⌝ ∗ is_allocator al bs true) 
+    }}}.
   Proof. 
-    iIntros (φ) "(%res&%cap&%Hr&%Hcr&%Hbs&#Hal2&Hal3&#Hal4&Hfl&Hfl2&Hun) Hphi". 
+    iIntros (Hr Hcr Hbs φ) "(#Hal2 & Hal3 & #Hal4 & Hfl & Hfl2 & Hun) Hphi". 
     iUnfold extend. wp_pures. wp_load. wp_load. wp_load. wp_pures. 
     destruct (decide (cap = 0)) as [Hc | Hc]. 
     { rewrite Hc. wp_pures. case_bool_decide; [|lia]. wp_pures. 
-      wp_apply ((freelist_extend_hoare al al res bs (al +ₗ 5) 0 0 0 0) with "[Hfl]"); 
+      wp_apply ((freelist_extend_hoare al al res bs true (al +ₗ 5) 0 0 0 0) with "[Hfl]"); 
       try lia; [by rewrite Z.mul_0_l|rewrite array_nil; iFrame "Hal2 Hal4 Hfl"|].
       rewrite Nat.sub_0_r Z.mul_0_l. destruct res; [lia|]. simpl. 
       rewrite replicate_add array_app. iDestruct "Hun" as "(Hun1 & Hun2)". 
-      iIntros "Hfl". wp_store. wp_pures. iApply "Hphi". iSplitL "Hal3 Hun2 Hfl Hfl2".
-      { rewrite length_replicate Z.add_0_l Z.add_0_r Loc.add_assoc. 
-        iFrame "Hal2 Hal4 Hfl Hfl2". iExists 1. iSplitR; [by iPureIntro|]. iSplitR; 
-        [iPureIntro; lia|]. iSplitR; [by iPureIntro|]. assert (S res - 1 = res) by lia.
-        rewrite Z.mul_1_l H0. by iSplitL "Hal3". }
-      iLeft. rewrite Z.mul_0_l !Z.add_0_r. iExists _. iSplitR; [done|]. iSplitL.
+      iIntros "Hfl". wp_store. wp_pures. iApply "Hphi". iLeft.
+      rewrite length_replicate Z.add_0_l Z.add_0_r Loc.add_assoc. 
+      iExists (al +ₗ 5). iSplitR; [done|]. iSplitL "Hun1".
       { iApply big_sepL_mono; [|by iApply seq_array_pointsto_eq]. iIntros. auto. }
-      iFrame "Hal4 Hal2". iExists 0. rewrite Z.mul_0_l. iPureIntro. split; [done|lia]. }
+      iSplitR. 
+      { iFrame "Hal2 Hal4". iExists 0. rewrite Z.mul_0_l Z.add_0_r. iPureIntro. 
+        split; [done|lia]. }
+      iFrame. iFrame "Hal2 Hal4". iExists 1, true, true. rewrite Z.mul_1_l.
+      replace (Z.of_nat 1) with (1%Z) by lia. replace (S res - 1) with (res) by lia. 
+      iFrame "Hal3 Hfl Hfl2 Hun2". iSplitR; [done|]. iSplitR; [done|]. iSplitR; [done|].
+      rewrite Nat.eqb_eq. iPureIntro. intuition. }
     case_bool_decide; [inv H; lia|]. wp_pures. case_bool_decide.
     { wp_pures. case_bool_decide; [inv H1; lia|]. wp_pures. 
       assert (Z.of_nat (cap - 1) = (Z.of_nat cap - 1)%Z) by lia. rewrite -H2.
@@ -243,95 +265,99 @@ Section Hoare.
       assert ((res - cap) * bs = (cap - 1) * bs + (res - cap - (cap - 1)) * bs) 
       by lia. rewrite H3 replicate_add array_app. 
       iDestruct "Hun" as "(Hun1 & Hun2)". rewrite length_replicate.
-      wp_apply (freelist_extend_hoare al al res bs (al +ₗ (5 + (cap * bs))) cap 
+      wp_apply (freelist_extend_hoare al al res bs true (al +ₗ (5 + (cap * bs))) cap 
       (cap - 1) 0 (cap - 1) with "[Hfl Hun1]"); try lia; [done| |].
       { iFrame "Hal2 Hfl Hal4". by rewrite Z.mul_0_l Loc.add_0. }
-      iIntros "Hfl". wp_store. wp_pures. iApply "Hphi".  
+      iIntros "Hfl". rewrite andb_true_l. wp_store. wp_pures. iApply "Hphi".  
       (*split: bs of *)
-      assert (res - cap - (cap - 1) = 1 + (res - cap - cap)) by lia. rewrite H4.
+      replace (res - cap - (cap - 1)) with (1 + (res - cap - cap)) by lia. 
       rewrite Nat.mul_add_distr_r Nat.mul_1_l replicate_add array_app.
-      iDestruct ("Hun2") as "(Hun1 & Hun2)". iSplitR "Hun1". 
-      { rewrite -Nat2Z.inj_add. iFrame "Hal2 Hal3 Hal4 Hfl Hfl2". iSplitR; 
-        [by iPureIntro|]. iSplitR; [iPureIntro; lia|]. iSplitR; [by iPureIntro|]. 
-        rewrite length_replicate !Loc.add_assoc. 
-        assert ((5 + cap * bs + (((cap - 1) * bs)%nat + bs))%Z 
-        = (5 + (cap + cap)%nat * bs)%Z) by lia.
-        assert ((res - cap - cap) * bs = (res - (cap + cap)) * bs) by lia.
-        by rewrite H5 H6. }
-      iLeft. rewrite Loc.add_assoc. 
-      assert ((5 + (cap + cap - 1) * bs)%Z = 
-      5 + cap * bs + ((cap - 1) * bs)%nat) by lia. rewrite H5. iExists _. 
-      iSplitR; [by iPureIntro|]. iSplitL. 
-      { iApply big_sepL_mono; [|iApply seq_array_pointsto_eq; iApply "Hun1"].
+      iDestruct ("Hun2") as "(Hun1 & Hun2)". iLeft. 
+      rewrite length_replicate !Loc.add_assoc. iExists _. iSplitR; [done|]. 
+      iSplitL "Hun1". 
+      { replace ((5 + (cap + cap - 1) * bs)%Z)  (*relies on earlier asserts*)
+        with (5 + cap * bs + ((cap - 1) * bs)%nat)%Z by lia. 
+        iApply big_sepL_mono; [|iApply seq_array_pointsto_eq; iApply "Hun1"].
         iIntros. iExists NONEV. 
-        assert ((5 + cap * bs + ((cap - 1) * bs)%nat)%Z = 
-        (5 + cap * bs + (cap - 1) * bs)%nat) by lia. by rewrite H7.  }
-      iFrame "Hal2 Hal4". iExists (cap + (cap - 1)). iPureIntro.
-      split; [|lia]. f_equal. lia. } 
+        by replace (5 + cap * bs + ((cap - 1) * bs)%nat)
+        with ((5 + cap * bs + (cap - 1) * bs)%nat) by lia. }
+      iSplitR. 
+      { iFrame "Hal2 Hal4". iExists (cap + cap - 1). Set Printing Coercions.
+        rewrite -Nat2Z.inj_add. iSplitR; [|iPureIntro; lia]. 
+        by replace (Z.of_nat (cap + cap) - 1)%Z with (Z.of_nat (cap + cap - 1)) by lia. }
+      rewrite -Nat2Z.inj_add. iFrame "Hfl2 Hal2 Hal3 Hal4 Hfl". iSplitR; [done|]. 
+      iSplitR; [iPureIntro; lia|]. iSplitR; [done|]. iSplitR. 
+      { iPureIntro. rewrite !Nat.eqb_eq. lia. }
+      assert ((5 + cap * bs + (((cap - 1) * bs)%nat + bs))%Z 
+      = (5 + (cap + cap)%nat * bs)%Z) by lia.
+      assert ((res - cap - cap) * bs = (res - (cap + cap)) * bs) by lia.
+      by rewrite -H4 H5 Z.add_assoc.  }
     wp_pures. destruct (decide (res - cap = 0)) as [Hcr2 | Hcr2]. 
     { rewrite -Nat2Z.inj_sub; [|done]. rewrite Hcr2. wp_pures. 
-      iApply "Hphi". iSplitL; [|by iRight].
-      iFrame "Hal2 Hal3 Hal4 Hfl Hfl2". iSplitR; [by iPureIntro|]. 
-      iSplitR; [by iPureIntro|]. iSplitR; [by iPureIntro|]. by rewrite Hcr2. }
+      iApply "Hphi". iRight. iSplitR; [done|]. iFrame "Hal2 Hal3 Hal4 Hfl Hfl2". 
+      iSplitR; [by iPureIntro|]. iSplitR; [by iPureIntro|]. iSplitR; 
+      [by iPureIntro|]. iSplitR; [|by rewrite Hcr2]. iPureIntro. 
+      intuition. lia. }
     case_bool_decide; [inv H1; lia|]. wp_pures.
     (* split (res - cap - 1) * bs + bs  *)
     assert (res - cap = (res - cap - 1) + 1) by lia. rewrite H2. 
     rewrite Nat.mul_add_distr_r Nat.mul_1_l replicate_add array_app length_replicate. 
     iDestruct "Hun" as "(Hun1 & Hun2)". 
-    iPoseProof (freelist_extend_hoare al al res bs (al +ₗ (5 + cap * bs)) 
+    iPoseProof (freelist_extend_hoare al al res bs true (al +ₗ (5 + cap * bs)) 
     cap (res - cap - 1) 0 (res - cap - 1)) as "H"; [lia|done|done|lia|done|]. 
     assert (Z.of_nat (res - cap - 1) = (Z.of_nat res - Z.of_nat cap - 1)%Z) by lia.
     rewrite H3. wp_apply ("H" with "[Hfl Hun1]"). 
     { rewrite Loc.add_assoc Z.mul_0_l Z.add_0_r. iFrame "Hfl Hun1 Hal2 Hal4". }
-    iIntros "Hfl". wp_store. wp_pures. iApply "Hphi". 
-    (* split bs of*) 
-    iSplitL "Hfl Hfl2 Hal3". 
-    { rewrite -Nat2Z.inj_sub; [|done]. rewrite -Nat2Z.inj_add. 
-      iFrame "Hal2 Hal3 Hal4 Hfl Hfl2". iSplitR; [by iPureIntro|]. iSplitR; 
-      [iPureIntro; lia|]. iSplitR; [by iPureIntro|].
-      assert (res - (cap + (res - cap)) = 0) by lia. rewrite H4 Nat.mul_0_l.
-      simpl. by rewrite array_nil. }
-    iLeft. rewrite !Loc.add_assoc. 
+    iIntros "Hfl". wp_store. wp_pures. iApply "Hphi". iLeft.
+    rewrite !Loc.add_assoc.
     assert ((5 + cap * bs + ((res - cap - 1) * bs)%nat)%Z 
     = (5 + (cap + (res - cap) - 1) * bs)%Z) by lia. rewrite H4. 
-    iExists _. iSplitR; [by iPureIntro|]. iSplitL.
+    iExists _. iSplitR; [by iPureIntro|]. iSplitL "Hun2".
     { iApply big_sepL_mono; [|by iApply seq_array_pointsto_eq]. iIntros. auto. }
-    iFrame "Hal2 Hal4". iExists (cap + (res - cap) - 1). iSplitR; [|iPureIntro; lia].
-    Set Printing Coercions. rewrite -Nat2Z.inj_sub; [|lia]. rewrite -Nat2Z.inj_add.
+    iSplitR. iFrame "Hal2 Hal4". iExists (cap + (res - cap) - 1). iSplitR; 
+    [|iPureIntro; lia]. rewrite -Nat2Z.inj_sub; [|lia]. rewrite -Nat2Z.inj_add.
     assert ((Z.of_nat (cap + (res - cap)) - 1)%Z 
     = (Z.of_nat (cap + (res - cap) - 1))%Z) by lia. by rewrite H5. 
+    iFrame "Hal2 Hal4". iExists (cap + (res - cap)). rewrite -Nat2Z.inj_sub; [|done]. 
+    rewrite -Nat2Z.inj_add. iFrame "Hal3 Hfl Hfl2". iSplitR; [by iPureIntro|]. 
+    iSplitR; [iPureIntro; lia|]. iSplitR; [by iPureIntro|]. iSplitR.
+    - iPureIntro. rewrite -H2 !Nat.eqb_eq. intuition; try lia.
+    - assert (res - (cap + (res - cap)) = 0) by lia. rewrite H5 Nat.mul_0_l.
+      simpl. by rewrite array_nil.
   Qed.
 
-  Lemma alloc_hoare al bs :
-    {{{ is_allocator al bs }}}
+  Lemma alloc_hoare al bs b :
+    {{{ is_allocator al bs b }}}
       alloc #al
     {{{ vret, RET vret; 
-      is_allocator al bs ∗
-      ((∃ l, ⌜vret = SOMEV #l⌝ ∗ ([∗ list] i ∈ seq 0 bs, ∃ v, (l +ₗ i) ↦ v) ∗ 
-        is_valid_loc l al)
+      (∃ l b', ⌜vret = SOMEV #l⌝ ∗ ([∗ list] i ∈ seq 0 bs, ∃ v, (l +ₗ i) ↦ v) ∗ 
+        is_valid_loc l al ∗ is_allocator al bs b')
         ∨ 
-      ⌜vret = NONEV⌝)
+      ⌜vret = NONEV⌝ ∗ is_allocator al bs true
     }}}.
   Proof.
-    iIntros (φ) "(%res&%cap&%Hr&%Hcr&%Hbs&#Hal2&Hal3&#Hal4&Hfl&Hfl2&Hun) Hphi". 
+    iIntros (φ) "(%res&%cap&%b1&%b2&%Hr&%Hcr&%Hbs&%Hf&#Hal2&Hal3&#Hal4&Hfl&Hfl2&Hun)Hphi".
     iUnfold alloc. wp_pures. 
     wp_apply (freelist_pop_hoare with "[Hfl]"); [iFrame "Hfl Hal4"|].
-    iIntros (v) "[(-> & Hfl) | (%l & -> & Hlbs & #Hlv & Hfl)]"; wp_pures.
+    iIntros (v) "[(-> & Hfl) | (%l & %b' & -> & Hlbs & #Hlv & Hfl)]"; wp_pures.
     { wp_apply (freelist_pop_hoare with "[Hfl2]"); [iFrame "Hfl2 Hal4"|].
-      iIntros (v) "[(-> & Hfl2) | (%l & -> & Hlbs & #Hlv & Hfl2)]"; wp_pures.
-      - wp_apply (extend_hoare with "[Hal3 Hun Hfl Hfl2]"); 
-        [iFrame "Hal2 Hal3 Hal4 Hfl2 Hfl Hun"; iPureIntro; lia|].
-        iIntros (v) "(Hal & [(%l & -> & Hlbs & #Hlv) | ->])"; iApply "Hphi"; 
-        [iFrame; iLeft; iFrame; auto|iFrame; by iRight]. 
-      - iDestruct "Hfl2" as "[Hal1 | (%l1 & %s1 & Hal1 & Hflr1)]"; wp_load; wp_store;
-        wp_store; wp_pures; iApply "Hphi". 
-        + iSplitR "Hlbs"; [|iLeft; by iFrame "Hlbs Hlv"]. 
-          iFrame. iFrame "Hal2 Hal4". iPureIntro; lia.
-        + iSplitR "Hlbs"; [|iLeft; by iFrame "Hlbs Hlv"]. 
-          iFrame "Hal2 Hal3 Hal4 Hun". iSplitR; [done|]. iSplitR; [done|].
-          iSplitR; [done|]. iSplitR "Hal1"; [iRight|iLeft]; by iFrame. } 
-    iApply "Hphi". iFrame. iSplitR; [iFrame "Hal2 Hal4"; iPureIntro; lia|].
-    iLeft. iFrame "Hlbs". by iSplitR. 
+      iIntros (v) "[(-> & Hfl2) | (%l & %b'' & -> & Hlbs & #Hlv & Hfl2)]"; wp_pures.
+      - wp_apply ((extend_hoare al res cap bs) with "[Hal3 Hun Hfl Hfl2]"); try lia; 
+        [iFrame; iFrame "Hal2 Hal4"|]. 
+        iIntros (v) "[(%l & -> & Hlbs & #Hvl & Hal) | (-> & Hal)]".
+        + iApply "Hphi". iLeft. iFrame "Hlbs Hal Hvl". done.
+        + iApply "Hphi". iRight. auto. 
+      - destruct b''; [|iDestruct "Hfl2" as "(%l1 & %s & Hal1 & Hflr)"]; wp_load; 
+        wp_store; wp_store; wp_pures; iApply "Hphi"; iLeft; iFrame "Hlbs Hlv".
+        + iExists (res =? cap). iSplitR; [done|]. iFrame. iExists true, true. 
+          iFrame "Hal2 Hal4 Hfl Hfl2". iSplitR; [done|]. iSplitR; [done|]. 
+          iSplitR; [done|]. iPureIntro. rewrite Nat.eqb_eq. tauto.
+        + iExists false. iSplitR; [done|]. iFrame. iExists false, true. 
+          iFrame "Hal1 Hal2 Hal4 Hfl Hflr". iSplitR; [done|]. iSplitR; [done|]. 
+          iSplitR; [done|]. iPureIntro. intuition; inversion H0. }
+    iApply "Hphi". iLeft. iFrame. iExists ((res =? cap) && b' && b2). 
+    iFrame "Hlv Hal2 Hal4". iSplitR; [done|]. iSplitR; [done|]. iSplitR; [done|]. 
+    iSplitR; [done|]. by rewrite !andb_true_iff Nat.eqb_eq Logic.and_assoc.
   Qed.
-
+ 
 End Hoare.
